\smalltitle{سوال 1}
\begin{enumerate}
    \item در حالت 0 همه‌ی مقدایر را صفر قرار می‌دهیم:
    \begin{gather*}
        V_0(s) = 0
    \end{gather*}
    حال برای بار اول داریم:
    \begin{align*}
        V_1(s_1) = \operatorname{max}(
            &0.6 \times 3 + 0.4 \times (-10),\\
            &1 \times (-1),\\
            &1 \times (-1)
        ) = -1\\
        V_1(s_2) = \operatorname{max}(
            &0.75 \times 2 + 0.25 \times (-10),\\
            &1 \times (-1),\\
            &1 \times (-1),\\
            &1 \times (-1)
        ) = -1\\
        V_1(s_3) = \operatorname{max}(
            &0.9 \times 2 + 0.1 \times (-10),\\
            &1 \times (-1),\\
            &1 \times (-1),\\
            &1 \times (-1)
        ) = 0.8\\
        V_1(s_4) = \operatorname{max}(
            &0.75 \times 2 + 0.25 \times (-10),\\
            &1 \times (-1),\\
            &1 \times (-1),\\
            &1 \times (-1)
        ) = -1\\
        V_1(s_5) = \operatorname{max}(
            &0.6 \times 3 + 0.4 \times (-10),\\
            &1 \times (-1),\\
            &1 \times (-1)
        ) = -1\\
        V_1(s_6) = \operatorname{max}(
            &0.6 \times 3 + 0.4 \times (-10),\\
            &1 \times (-1),\\
            &1 \times (-1)
        ) = -1\\
        V_1(s_7) = \operatorname{max}(
            &0.75 \times 2 + 0.25 \times (-10),\\
            &1 \times (-1),\\
            &1 \times (-1),\\
            &1 \times (-1)
        ) = -1\\
        V_1(s_8) = \operatorname{max}(
            &0.75 \times 2 + 0.25 \times (-10),\\
            &1 \times (-1),\\
            &1 \times (-1),\\
            &1 \times (-1)
        ) = -1\\
        V_1(s_9) = \operatorname{max}(
            &0.75 \times 2 + 0.25 \times (-10),\\
            &1 \times (-1),\\
            &1 \times (-1),\\
            &1 \times (-1)
        ) = -1\\
        V_1(s_{10}) = \operatorname{max}(
            &0.6 \times 3 + 0.4 \times (-10),\\
            &1 \times (-1),\\
            &1 \times (-1)
        ) = -1
    \end{align*}
    برای بار دوم نیز به توجه به حالت اول داریم:
    \begin{align*}
        V_2(s_1) = \operatorname{max}(
            &0.6 \times 3 + 0.4 \times (-10),\\
            &1 \times (-1 - 1),\\
            &1 \times (-1 - 1)
        ) = -2\\
        V_2(s_2) = \operatorname{max}(
            &0.75 \times 2 + 0.25 \times (-10),\\
            &1 \times (-1 - 1),\\
            &1 \times (-1 + 0.8),\\
            &1 \times (-1 - 1)
        ) = -0.2\\
        V_2(s_3) = \operatorname{max}(
            &0.9 \times 2 + 0.1 \times (-10),\\
            &1 \times (-1 - 1),\\
            &1 \times (-1 - 1),\\
            &1 \times (-1 - 1)
        ) = 0.8\\
        V_2(s_4) = \operatorname{max}(
            &0.75 \times 2 + 0.25 \times (-10),\\
            &1 \times (-1 - 1),\\
            &1 \times (-1 + 0.8),\\
            &1 \times (-1 - 1)
        ) = -0.2\\
        V_2(s_5) = \operatorname{max}(
            &0.6 \times 3 + 0.4 \times (-10),\\
            &1 \times (-1 - 1),\\
            &1 \times (-1 - 1)
        ) = -2\\
        V_2(s_6) = \operatorname{max}(
            &0.6 \times 3 + 0.4 \times (-10),\\
            &1 \times (-1 - 1),\\
            &1 \times (-1 - 1)
        ) = -2\\
        V_2(s_7) = \operatorname{max}(
            &0.75 \times 2 + 0.25 \times (-10),\\
            &1 \times (-1 - 1),\\
            &1 \times (-1 - 1),\\
            &1 \times (-1 - 1)
        ) = -1\\
        V_2(s_8) = \operatorname{max}(
            &0.75 \times 2 + 0.25 \times (-10),\\
            &1 \times (-1 - 1),\\
            &1 \times (-1 + 0.8),\\
            &1 \times (-1 - 1)
        ) = 0.2\\
        V_2(s_9) = \operatorname{max}(
            &0.75 \times 2 + 0.25 \times (-10),\\
            &1 \times (-1 - 1),\\
            &1 \times (-1 - 1),\\
            &1 \times (-1 - 1)
        ) = -1\\
        V_2(s_{10}) = \operatorname{max}(
            &0.6 \times 3 + 0.4 \times (-10),\\
            &1 \times (-1 - 1),\\
            &1 \times (-1 - 1)
        ) = -2
    \end{align*}
    \item 
\end{enumerate}








